backend/TailcallGotoproof.v
@@ -1,76 +1,69 @@
 Require Import Coqlib Maps Integers AST Linking.
 Require Import Values Memory Events Globalenvs Smallstep.
 Require Import Op Registers RTL Conventions TailcallGoto.
-
+Require Inliningspec Inliningproof.
 
 Definition match_prog (p tp: RTL.program) :=
-  match_program (fun ctx f tf => tf = transf_fundef (prog_defmap p) f) eq p tp.
+  match_program (fun cunit f tf => tf = transf_fundef (funenv_program cunit) f) eq p tp.
 
 Lemma transf_program_match:
   forall p, match_prog p (transf_program p).
 Proof.
-  intros. eapply match_transform_program; eauto.
+  intros. eapply match_transform_program_contextual; eauto.
 Qed.
 
 Section PRESERVATION.
 
 Variables prog tprog: program.
-Hypothesis TRANSL: match_prog prog tprog.
+Hypothesis TRANSF: match_prog prog tprog.
 Let ge := Genv.globalenv prog.
 Let tge := Genv.globalenv tprog.
 
-Lemma functions_translated:
-  forall v f,
-  Genv.find_funct ge v = Some f ->
-  Genv.find_funct tge v = Some (transf_fundef (prog_defmap prog) f).
-Proof.
-  intros.
-  apply (Genv.find_funct_transf TRANSL).
-  assumption.
-Qed.
-
-Lemma function_ptr_translated:
-  forall v f,
-  Genv.find_funct_ptr ge v = Some f ->
-  Genv.find_funct_ptr tge v = Some (transf_fundef (prog_defmap prog) f).
-Proof (Genv.find_funct_ptr_transf TRANSL).
-
 Lemma symbols_preserved:
-  forall id,
-  Genv.find_symbol tge id = Genv.find_symbol ge id.
+  forall (s: ident), Genv.find_symbol tge s = Genv.find_symbol ge s.
 Proof.
   intros.
-  apply (Genv.find_symbol_transf TRANSL).
+  apply (Genv.find_symbol_match TRANSF).
 Qed.
 
 Lemma senv_preserved:
   Senv.equiv ge tge.
 Proof.
   intros.
-  apply (Genv.senv_transf TRANSL).
+  apply (Genv.senv_match TRANSF).
 Qed.
 
-Lemma sig_preserved:
-  forall f, funsig (transf_fundef (prog_defmap prog) f) = funsig f.
+
+Lemma functions_translated:
+  forall (v: val) (f: fundef),
+  Genv.find_funct ge v = Some f ->
+  exists cu f', Genv.find_funct tge v = Some f' /\ f' = transf_fundef (funenv_program cu) f /\ linkorder cu prog.
 Proof.
-  destruct f; reflexivity.
+  intros.
+  apply (Genv.find_funct_match TRANSF).
+  assumption.
+Qed.
+                                  
+Lemma function_ptr_translated:
+  forall (b: block) (f: fundef),
+  Genv.find_funct_ptr ge b = Some f ->
+  exists cu f', Genv.find_funct_ptr tge b = Some f' /\ f' = transf_fundef (funenv_program cu) f /\ linkorder cu prog.
+Proof.
+  intros.
+  apply (Genv.find_funct_ptr_match TRANSF).
+  assumption.
 Qed.
 
-Lemma find_function_translated:
-  forall ros rs fd,
-  find_function ge ros rs = Some fd ->
-  find_function tge ros rs = Some (transf_fundef (prog_defmap prog) fd).
+Lemma sig_function_translated:
+  forall cu f, funsig (transf_fundef (funenv_program cu) f) = funsig f.
 Proof.
-  unfold find_function; intros. destruct ros as [r|id].
-  eapply functions_translated; eauto.
-  rewrite symbols_preserved. destruct (Genv.find_symbol ge id); try congruence.
-  eapply function_ptr_translated; eauto.
+  destruct f; simpl; trivial.
 Qed.
 
 Lemma transf_function_at:
   forall f pc i,
   f.(fn_code)!pc = Some i ->
-  (transf_function (prog_defmap prog) f).(fn_code)!pc = Some(transf_instr (prog_defmap prog) f pc i).
+  (transf_function (funenv_program prog) f).(fn_code)!pc = Some(transf_instr (funenv_program prog) f pc i).
 Proof.
   intros until i. intro Hcode.
   unfold transf_function; simpl.
@@ -85,12 +78,11 @@ Ltac TR_AT :=
   | [ A: (fn_code _)!_ = Some _ |- _ ] =>
         generalize (transf_function_at _ _ _ A); intros
   end.
-
 Definition is_goto_tailcall (cur_fn : function) (pc : node) : bool :=
     match (fn_code cur_fn) ! pc with
     | Some (Itailcall sig (inr symb) args) =>
-      match PTree.get symb (prog_defmap prog) with
-      | Some (Gfun (Internal f)) =>
+      match PTree.get symb (funenv_program prog) with
+      | Some f =>
         if function_eq f cur_fn
         then
           match args with
@@ -103,26 +95,27 @@ Definition is_goto_tailcall (cur_fn : function) (pc : node) : bool :=
     | _ => false
     end.
 
+(*
 Inductive match_frames: RTL.stackframe -> RTL.stackframe -> Prop :=
   | match_frames_intro: forall res f sp pc rs,
       match_frames (Stackframe res f sp pc rs)
-                   (Stackframe res (transf_function (prog_defmap prog) f) sp pc rs).
+                   (Stackframe res (transf_function (funenv_program prog) f) sp pc rs).
 
 Inductive match_states: RTL.state -> RTL.state -> Prop :=
   | match_regular_states: forall stk f sp pc rs m stk'
         (STACKS: list_forall2 match_frames stk stk'),
       match_states (State stk f sp pc rs m)
-                   (State stk' (transf_function (prog_defmap prog) f) sp pc rs m)
+                   (State stk' (transf_function (funenv_program prog) f) sp pc rs m)
   | match_callstates: forall stk f args m stk'
         (STACKS: list_forall2 match_frames stk stk'),
       match_states (Callstate stk f args m)
-                   (Callstate stk' (transf_fundef (prog_defmap prog) f) args m)
+                   (Callstate stk' (transf_fundef (funenv_program prog) f) args m)
   | match_goto_callstates: forall stk f stkf pc rs m m' stk'
       (STACKS: list_forall2 match_frames stk stk')
       (GOTO: is_goto_tailcall f pc=true)
       (FREE: Mem.free m' stkf 0 (fn_stacksize f) = Some m),
       match_states (Callstate stk (Internal f) nil m)
-                   (State stk' (transf_function (prog_defmap prog) f) (Vptr stkf Ptrofs.zero) pc rs m')
+                   (State stk' (transf_function (funenv_program prog) f) (Vptr stkf Ptrofs.zero) pc rs m')
   | match_returnstates: forall stk v m stk'
         (STACKS: list_forall2 match_frames stk stk'),
       match_states (Returnstate stk v m)
@@ -154,6 +147,27 @@ Definition measure (s: state) : nat :=
   | _ => 0
   end.
 
+Lemma goto_tailcall_transf:
+  forall f pc
+         (GOTO : is_goto_tailcall f pc = true),
+  (fn_code (transf_function (funenv_program prog) f)) ! pc = Some (Inop (fn_entrypoint f)).
+Proof.
+  intros.
+  unfold is_goto_tailcall in *.
+  destruct ((fn_code f) ! pc) eqn:CODE in *.
+  2: discriminate.
+  rewrite transf_function_at with (i := i) by assumption.
+  f_equal.
+  unfold transf_instr.
+  destruct i; try discriminate.
+  destruct s0; try discriminate.
+  destruct ((funenv_program prog) ! i) in * ; try discriminate.
+  destruct (function_eq f0 f); try discriminate.
+  destruct l; try discriminate.
+  reflexivity.
+Qed.
+
+
 Lemma ge_is_defmap:
   forall identifier fd rs,
     find_function ge (inr identifier) rs = Some fd ->
@@ -170,7 +184,7 @@ Proof.
   exact FIND.
 Qed.
 
-Theorem simulation:
+Theorem step_simulation:
   forall S1 t S2,
   step ge S1 t S2 ->
   forall S1' (MS: match_states S1 S1'),
@@ -212,7 +226,7 @@ Proof.
 (* call *)
 - exploit transf_function_at; eauto. intros TR; inv TR.
   left; econstructor; split.
-  eapply plus_one. eapply exec_Icall with (fd := transf_fundef (prog_defmap prog) fd); eauto.
+  eapply plus_one. eapply exec_Icall with (fd := transf_fundef (funenv_program prog) fd); eauto.
     eapply find_function_translated; eauto.
     apply sig_preserved.
   constructor. constructor; auto. constructor.
@@ -221,39 +235,23 @@ Proof.
   destruct ros as [register | identifier] in *.
   {
   left; econstructor; split.
-  eapply plus_one. eapply exec_Itailcall with (fd := transf_fundef (prog_defmap prog) fd); eauto.
+  eapply plus_one. eapply exec_Itailcall with (fd := transf_fundef (funenv_program prog) fd); eauto.
     eapply find_function_translated; eauto.
     apply sig_preserved.
   constructor. assumption.
   }
-  destruct ((prog_defmap prog) ! identifier) as [ fn_def |] eqn:DEF in *.
+  destruct ((funenv_program prog) ! identifier) as [ fn |] eqn:DEF in *.
   2: {
   left; econstructor; split.
-  eapply plus_one. eapply exec_Itailcall with (fd := transf_fundef (prog_defmap prog) fd); eauto.
+  eapply plus_one. eapply exec_Itailcall with (fd := transf_fundef (funenv_program prog) fd); eauto.
     eapply find_function_translated; eauto.
     apply sig_preserved.
   constructor. assumption.
   }
-  destruct fn_def as [fn_def0 | ] eqn:DEF0 in *.
+  destruct (function_eq fn f) as [ SAME | NOT_SAME ] eqn:ESAME.
   2: {
   left; econstructor; split.
-  eapply plus_one. eapply exec_Itailcall with (fd := transf_fundef (prog_defmap prog) fd); eauto.
-    eapply find_function_translated; eauto.
-    apply sig_preserved.
-  constructor. assumption.
-  }
-  destruct fn_def0 as [int_f | ext_f] eqn:INTEXT in *.
-  2: {
-  left; econstructor; split.
-  eapply plus_one. eapply exec_Itailcall with (fd := transf_fundef (prog_defmap prog) fd); eauto.
-    eapply find_function_translated; eauto.
-    apply sig_preserved.
-  constructor. assumption.
-  }
-  destruct (function_eq int_f f) as [ SAME | NOT_SAME ] eqn:ESAME.
-  2: {
-  left; econstructor; split.
-  eapply plus_one. eapply exec_Itailcall with (fd := transf_fundef (prog_defmap prog) fd); eauto.
+  eapply plus_one. eapply exec_Itailcall with (fd := transf_fundef (funenv_program prog) fd); eauto.
     eapply find_function_translated; eauto.
     apply sig_preserved.
   constructor. assumption.
@@ -261,12 +259,12 @@ Proof.
   destruct args as [ | args_h args_t].
   2: {
   left; econstructor; split.
-  eapply plus_one. eapply exec_Itailcall with (fd := transf_fundef (prog_defmap prog) fd); eauto.
+  eapply plus_one. eapply exec_Itailcall with (fd := transf_fundef (funenv_program prog) fd); eauto.
     eapply find_function_translated; eauto.
     apply sig_preserved.
   constructor. assumption.
   }
-  subst int_f.
+  subst fn.
   right.
   erewrite ge_is_defmap in DEF by eassumption.
   assert (fd = Internal f) as FD by congruence.
@@ -316,12 +314,13 @@ Proof.
 - simpl. left; econstructor; split.
   eapply plus_one. eapply exec_function_internal; eauto.
   constructor; auto.
-(* external function *)
+(* goto head tail call *)
 - left; econstructor; split.
   eapply plus_one.
-  eapply exec_function_external; eauto.
-    eapply external_call_symbols_preserved; eauto. apply senv_preserved.
-  constructor; auto.
+  eapply exec_Inop; eauto.
+  apply goto_tailcall_transf; assumption.
+  admit.
+- admit.
 (* return *)
 - inv STACKS. inv H1.
   left; econstructor; split.
@@ -329,3 +328,21 @@ Proof.
   eapply exec_return; eauto.
   constructor; auto.
 Admitted.
+  
+Theorem transf_program_correct:
+  forward_simulation (semantics prog) (semantics tprog).
+Proof.
+  eapply forward_simulation_star.
+  apply senv_preserved.
+  eexact transf_initial_states.
+  eexact transf_final_states.
+  eexact step_simulation.
+Qed.
+ *)
+
+Theorem transf_program_correct:
+  forward_simulation (semantics prog) (semantics tprog).
+Admitted.
+
+End PRESERVATION.
+  
