Makefile
@@ -76,7 +76,7 @@ BACKEND=\
   Registers.v RTL.v \
   RTLgen.v RTLgenspec.v RTLgenproof.v \
   Tailcall.v Tailcallproof.v \
-  TailcallGoto.v \
+  TailcallGoto.v TailcallGotoproof.v \
   Inlining.v Inliningspec.v Inliningproof.v \
   Renumber.v Renumberproof.v \
   RTLtyping.v \
